temp:Memory model for SMS

common/Memstructure.v
@@ -127,128 +127,810 @@ Opaque MemPos.alloc MemPos.free MemPos.store MemPos.load MemPos.storebytes MemPo
   MemPos.unchanged_on_refl
 : mem.
 
-(* Module Type SUP(Block:BLOCK).
-Include Block.
-Parameter sup: Type.
+(** * Difinition of Nominal Memory Model with Structured Memory Space **)
 
-Parameter sup_empty : sup.
+Definition path := list nat.
 
-Parameter sup_In : block -> sup -> Prop.
-Parameter empty_in: forall b, ~ sup_In b sup_empty.
-Parameter sup_dec : forall b s, {sup_In b s}+{~sup_In b s}.
+Definition fid := option ident. (*None means external function*)
 
-Parameter fresh_block : sup -> block.
-Parameter freshness : forall s, ~sup_In (fresh_block s) s.
-
-Parameter sup_add : block -> sup -> sup.
-
-Definition sup_incr(s:sup) := sup_add (fresh_block s) s.
-
-Definition sup_include(s1 s2:sup) := forall b, sup_In b s1 -> sup_In b s2.
-
-Parameter sup_add_in : forall b s b', sup_In b' (sup_add b s) <-> b' = b \/ sup_In b' s.
-
-Theorem sup_add_in1 : forall b s, sup_In b (sup_add b s).
-Proof. intros. apply sup_add_in. left. auto. Qed.
-Theorem sup_add_in2 : forall b s, sup_include s (sup_add b s).
-Proof. intros. intro. intro. apply sup_add_in. right. auto. Qed.
-
-Lemma sup_include_refl : forall s:sup, sup_include s s.
-Proof. intro. intro. auto. Qed.
-
-Lemma sup_include_trans:
-  forall p q r:sup,sup_include p q-> sup_include q r -> sup_include p r.
+Lemma nat_eq: forall n1 n2 :nat, {n1=n2} + {n1<>n2}.
 Proof.
-  intros. intro. intro.  auto.
+  intros.
+  destruct (Nat.eqb n1 n2) eqn:?.
+  apply Nat.eqb_eq in Heqb. left. auto.
+  apply Nat.eqb_neq in Heqb. right. auto.
 Qed.
 
-Lemma sup_include_incr:
-  forall s b, sup_include s (sup_add b s).
+Lemma beq : forall b1 b2:bool, {b1=b2}+{b1<>b2}.
 Proof.
-  intros. apply sup_add_in2.
+  intros.
+  destruct (eqb b1 b2) eqn:?.
+  rewrite eqb_true_iff in Heqb. auto.
+  rewrite eqb_false_iff in Heqb. auto.
 Qed.
 
-End SUP.*)
-(* WIP: 3part mem
-Module Memstructure1.
+Definition eq_path := list_eq_dec nat_eq.
 
-Module Block <: BLOCK.
+Definition fid_eq : forall fi1 fi2 : fid, {fi1=fi2} + {fi1<>fi2}.
+Proof.
+  intros.
+  destruct fi1; destruct fi2.
+  + destruct (peq i i0). left. congruence. right. congruence.
+  + right. congruence.
+  + right. congruence.
+  + left. congruence.
+Qed.
+
+Module Struc_Block <: BLOCK.
+
 Inductive block' :=
-|Global : ident -> block'
-|Heap : ident -> block'
-|Stack : ident -> block'.
+  |Stack : fid -> path -> positive -> block'
+  |Global : ident -> block'.
 
 Definition block := block'.
+
 Theorem eq_block : forall (x y:block),{x=y}+{x<>y}.
 Proof.
-  intros. destruct x; destruct y.
-  destruct (peq i i0). left; congruence. right; congruence.
-  right. congruence. right. congruence.
-  right. congruence.
-  destruct (peq i i0). left; congruence. right; congruence.
-  right. congruence.
-  right. congruence. right. congruence.
-  destruct (peq i i0). left; congruence. right; congruence.
+  intros. destruct x; destruct y; try(right; congruence).
+  - (destruct (eq_path p p1)); try (right; congruence).
+    destruct (peq p0 p2); try (right; congruence).
+    destruct (fid_eq f f0). left. congruence. right. congruence.
+  - destruct (peq i i0). left. congruence. right. congruence.
 Qed.
-End Block.
 
-Module Mem := Mem(Block).
-Include Block.
+End Struc_Block.
 
-Record structure := mk_struc{
- global_sup: list ident;
- heap_sup: list ident;
- stack_sup: list ident;
-}.
+Section STREE.
 
-Definition structure_In (b:block)(s:structure) :=
-  match b with
-    |Global id => In id (global_sup s)
-    |Heap id => In id (heap_sup s)
-    |Stack id => In id (stack_sup s)
-  end.
-
-
-Definition match_mem_structure (m:MemPos.mem) (s:structure) :=
-   forall b, Mem.valid_block m b <-> structure_In b s.
-
-Fixpoint find_max_pos (l: list positive) : positive :=
+Fixpoint fresh_pos (l: list positive) : positive :=
   match l with
   |nil => 1
-  |hd::tl => let m' := find_max_pos tl in
+  |hd::tl => let m' := fresh_pos tl in
              match plt hd m' with
              |left _ => m'
-             |right _ => hd
+             |right _ => hd +1
              end
   end.
 
-Theorem Lessthan: forall p l, In p l -> Ple p (find_max_pos l).
+Lemma Lessthan: forall b l, In b l -> Plt b (fresh_pos l).
 Proof.
   intros.
   induction l.
   destruct H.
   destruct H;simpl.
-  - destruct (plt a (find_max_pos l)); subst a.
-    + apply Plt_Ple. assumption.
-    + apply Ple_refl.
-  - destruct (plt a (find_max_pos l)); apply IHl in H.
+  - destruct (plt a (fresh_pos l)); subst a.
+    auto.
+    apply Pos.lt_add_r.
+  - destruct (plt a (fresh_pos l)); apply IHl in H.
     + auto.
-    + eapply Ple_trans. eauto.  apply Pos.le_nlt. apply n.
+    + eapply Plt_trans. eauto.
+      apply Pos.le_nlt in n.
+
+      apply Pos.le_lteq in n. destruct n.
+      eapply Plt_trans. eauto.
+      apply Pos.lt_add_r.
+      subst.
+      apply Pos.lt_add_r.
 Qed.
 
-Definition fresh_ident (l: list ident ) := Pos.succ (find_max_pos l).
 
-Theorem freshness : forall s, ~In (fresh_ident s) s.
+Lemma fresh_notin : forall l, ~In (fresh_pos l) l.
 Proof.
-  intros. unfold fresh_ident.
-  intro.
-  apply Lessthan in H.
-  assert (Plt (find_max_pos s) (Pos.succ (find_max_pos s))). apply Plt_succ.
-  assert (Plt (find_max_pos s) (find_max_pos s)). eapply Plt_Ple_trans. eauto. auto.
-  apply Plt_strict in H1.
-  auto.
+  intros. intro. apply Lessthan in H.
+  unfold fresh_pos in H. extlia.
 Qed.
 
-End Memstructure1.
-*)
+Import List.ListNotations.
+
+Inductive stree : Type :=
+  |Node : fid -> (list positive)  -> list stree -> option stree -> stree.
+
+Fixpoint cdepth (t:stree) : nat :=
+  match t with
+    |Node fid bl tl (Some hd) => S (cdepth hd)
+    |Node fid bl tl None => O
+  end.
+
+(* well-founded induction *)
+
+Fixpoint depth (t:stree) : nat :=
+  match t with
+    |Node fid bl tl head =>
+     let d_head := option_map depth head in
+     let d_list := map depth tl in
+     let f := (fun n1 n2 => if Nat.leb n1 n2 then n2 else n1) in
+     match d_head with
+       |None => fold_right f O d_list + 1
+       |Some n => fold_right f n d_list + 1
+     end
+  end.
+
+Definition substree (t1 t2 : stree) : Prop :=
+  match t2 with
+    |Node fid bl tl head => head = Some t1 \/ In t1 tl end.
+
+Lemma substree_depth : forall t1 t2, substree t1 t2 ->
+                                ((depth t1) < (depth t2))%nat.
+Proof.
+  intros. unfold substree in H. destruct t2.
+  inv H.
+  - simpl. induction l0.
+    + simpl. lia.
+    + simpl. destr. apply Nat.leb_gt in Heqb. lia.
+  - induction l0.
+    + inv H0.
+    + inv H0.
+      simpl. repeat destr.
+      apply Nat.leb_le in Heqb. lia.
+      apply Nat.leb_gt in Heqb. lia.
+      apply Nat.leb_le in Heqb. lia.
+      apply Nat.leb_gt in Heqb. lia.
+      apply IHl0 in H. simpl in *.
+      repeat destr.
+      apply Nat.leb_gt in Heqb. lia.
+      apply Nat.leb_gt in Heqb. lia.
+Qed.
+
+Lemma substree_wf' : forall n t, (depth t <= n)%nat -> Acc substree t.
+  unfold substree; induction n; intros.
+  - destruct t.
+    destruct o; destruct l0.
+    + simpl in H. extlia.
+    + simpl in H. extlia.
+    + constructor. intros. inv H0; inv H1.
+    + simpl in H. extlia.
+  - constructor.
+    intros.
+    apply substree_depth in H0.
+    apply IHn. lia.
+Defined.
+
+Lemma substree_wf : well_founded substree.
+  red; intro. eapply substree_wf'; eauto.
+Defined.
+
+Definition stree_ind := well_founded_induction substree_wf.
+
+(* operations *)
+Definition empty_stree := Node None [] [] None.
+
+Fixpoint next_stree (t: stree) (id:ident) : (stree * path) :=
+  match t with
+  | Node b bl l None =>
+    let idx := length l in
+    ((Node b bl l (Some (Node (Some id) [] [] None))), [idx])
+  | Node b bl l (Some t') =>
+    let (t'', p) := next_stree t' id in
+    (Node b bl l (Some t''), (length l) :: p)
+  end.
+
+Fixpoint next_block_stree (t:stree) : (fid * positive * path * stree) :=
+  match t with
+  |Node b bl l None =>
+   (b, (fresh_pos bl), nil, Node b ((fresh_pos bl)::bl) l None)
+  |Node b bl l (Some t') =>
+   match next_block_stree t' with (pos,path,t'')
+    => (pos, (length l)::path, Node b bl l (Some t''))
+   end
+  end.
+
+Fixpoint return_stree (t: stree) : option (stree * path):=
+  match t with
+  | Node _ bl l None =>
+    None
+  | Node b bl l (Some t) =>
+    let idx := length l in
+    match return_stree t with
+    | None => Some ((Node b bl (l ++ [t]) None),[idx])
+    | Some (t',p') => Some ((Node b bl l (Some t')),(idx::p'))
+    end
+  end.
+
+Fixpoint stree_In (fid:option ident)(p:path) (pos:positive) (t:stree) :=
+  match p,t with
+    |nil , Node b' bl dt _ => fid = b' /\ In pos bl
+    |n::p' , Node b' bl dt None =>
+     match nth_error dt n with
+       |Some t' => stree_In fid p' pos t'
+       |None => False
+     end
+    |n::p',Node b' bl dt (Some t') =>
+     if (n =? (length dt))%nat then stree_In fid p' pos t' else
+     match nth_error dt n with
+       |Some t'' => stree_In fid p' pos t''
+       |None => False
+     end
+  end.
+
+Lemma node_Indec :
+  forall (f f0:fid) (p:positive) (l: list positive), {f=f0 /\ In p l}+{~(f=f0/\ In p l)}.
+Proof.
+  intros.
+  destruct (fid_eq f f0) eqn:?.
+  destruct (In_dec peq p l).
+  subst. auto.
+  right. intro. inv H. congruence.
+  right. intro. inv H. congruence.
+Qed.
+
+(* properties of the operations above *)
+
+Definition cpath (s:stree) : path :=
+  match next_block_stree s with
+    |(f,pos,path,_) => path
+  end.
+
+Definition npath (s:stree)(id:ident) : path :=
+  let (t,p) := next_stree s id in p.
+
+Lemma next_stree_cdepth: forall p t t' id,
+    next_stree t id = (t',p) -> cdepth t' = S (cdepth t).
+Proof.
+  induction p; (intros; destruct t; destruct o; simpl in H).
+  destr_in H. inv H. destr_in H. inv H.
+  simpl. exploit IHp; eauto. inv H. simpl. auto.
+Qed.
+
+Lemma next_block_stree_cdepth : forall p pos fid t t',
+    next_block_stree t = (fid,pos,p,t') -> cdepth t' = cdepth t.
+Proof.
+  induction p; (intros; destruct t; destruct o; inv H; repeat destr_in H1).
+  auto. simpl. exploit IHp; eauto.
+Qed.
+
+Lemma return_stree_cdepth : forall p t t',
+    return_stree t = Some (t',p) -> S (cdepth t') = (cdepth t).
+Proof.
+  induction p; (intros; destruct t; destruct o; inv H; repeat destr_in H1).
+  simpl. exploit IHp; eauto. simpl. destruct s. destruct o.
+  simpl in Heqo. repeat destr_in Heqo. reflexivity.
+Qed.
+
+Lemma next_stree_cpath :
+  forall p t t' id,
+    next_stree t id = (t',p) ->  cpath t' = p.
+Proof.
+  induction p.
+  - intros. destruct t. destruct o.
+    simpl in H. destruct (next_stree s id). inv H.
+    simpl in H. inv H.
+  - intros. destruct t. destruct o.
+    simpl in H. destruct (next_stree s id) eqn:?. inv H.
+    apply IHp in Heqp0.
+    unfold cpath in *. simpl in *.
+    destruct (next_block_stree s0) eqn:?.
+    destruct p0 eqn:?.
+    destruct p1 eqn:?.
+    congruence. simpl in H. inv H.
+    unfold cpath. simpl. auto.
+Qed.
+
+Lemma next_stree_next_block_stree :
+  forall t t' t'' id p f pos path,
+    next_stree t id = (t',p) ->
+    next_block_stree t' = (f,pos,path,t'') ->
+    f = Some id /\ pos = 1%positive /\ path = p.
+Proof.
+  induction t using stree_ind. intros. destruct t. destruct o.
+  - simpl in H0. destruct (next_stree s id) eqn:?. inv H0. simpl in H1.
+    destruct (next_block_stree s0) eqn:?. destruct p. destruct p.
+    exploit H. instantiate (1:=s). simpl. auto. eauto. eauto. inv H1.
+    intros [A [B C]]. split. auto. split. auto. congruence.
+  - simpl in H0. inv H0. simpl in H1. inv H1. auto.
+Qed.
+
+Lemma next_block_stree_next_block : forall s1 s2 s3 fid1 fid2 pos1 pos2 path1 path2,
+      next_block_stree s1 = (fid1,pos1,path1,s2) ->
+      next_block_stree s2 = (fid2,pos2,path2,s3) ->
+      fid1 = fid2 /\ path1 = path2 /\ pos2 = Pos.succ pos1.
+Proof.
+  induction s1 using stree_ind. intros. destruct s1. destruct o.
+  - simpl in H0. destruct (next_block_stree s) eqn:?. destruct p. destruct p.
+    inv H0. simpl in H1.
+    destruct (next_block_stree s0) eqn:?. destruct p. destruct p. inv H1.
+    exploit H. instantiate (1:=s). simpl. auto. eauto. eauto.
+    intros [A [B C]]. split. auto. split. rewrite B. auto. auto.
+  - simpl in H0. inv H0. simpl in H1. inv H1. split. auto.
+    split. auto. rewrite pred_dec_false. lia. extlia.
+Qed.
+
+Definition stree_Indec :forall tree f path p , {stree_In f path p tree}+{~stree_In f path p tree}.
+Proof.
+  induction tree using (well_founded_induction substree_wf ); intros.
+  destruct tree; destruct path0.
+  - simpl. apply node_Indec.
+  - destruct o; destruct l0; simpl; repeat destr.
+    + apply H. simpl. auto.
+    + rewrite nth_error_nil in Heqo. congruence.
+    + apply H. simpl. auto.
+    + apply nth_error_in in Heqo.
+      apply H. simpl. auto.
+    + rewrite nth_error_nil in Heqo. congruence.
+    + apply nth_error_in in Heqo.
+      apply H. simpl. auto.
+Qed.
+
+Lemma stree_freshness : forall b p pos t t', next_block_stree t = (b,pos,p,t')
+  -> ~ stree_In b p pos t.
+Proof.
+  induction p.
+  - intros. destruct t. simpl in *.
+    destruct o.
+    destruct (next_block_stree s).
+    destruct p. inv H.
+    inv H.
+    intro. inv H. apply fresh_notin in H1. auto.
+  - intros. destruct t. simpl in *.
+    destruct o.
+    destruct (next_block_stree s) eqn:?.
+    destruct p0. inv H.
+    rewrite <- beq_nat_refl. eauto.
+    inv H.
+Qed.
+
+Lemma next_block_stree_in : forall t t' path pos path' pos' f f',
+        next_block_stree t = (f,pos,path,t') ->
+        stree_In f' path' pos' t' <->
+        ((f',path',pos') = (f,path,pos)
+        \/ stree_In f' path' pos' t).
+Proof.
+  induction t using stree_ind. intros.
+  destruct t.
+  - destruct path0; destruct path';
+    simpl in H0; repeat destr_in H0; simpl.
+    + split; intros; inv H0.
+      inv H2; auto.
+      inv H1; auto. inv H1; auto.
+    + split; intros; auto.
+      destruct H0. inv H0. auto.
+    + split; intros; auto.
+      destruct H0. inv H0. auto.
+    + destr.
+      *
+      apply beq_nat_true in Heqb. subst.
+      exploit H; eauto. simpl. auto.
+      intros.
+      split; intros. apply H0 in H1.
+      inv H1. left. inv H2. auto.
+      right. auto.
+      apply H0. inv H1. inv H2. auto.
+      auto.
+      *
+      apply beq_nat_false in Heqb.
+      destr.
+Qed.
+
+Lemma next_stree_in : forall p p' t t' pos b id,
+    next_stree t id = (t',p') ->
+    stree_In b p pos t <-> stree_In b p pos t'.
+Proof.
+  induction p.
+  - intros. destruct t. destruct o.
+    simpl in H. destruct (next_stree s). inv H.
+    simpl. reflexivity.
+    simpl in H. inv H.
+    simpl. reflexivity.
+  - intros. destruct t. destruct o.
+    * simpl in H. destruct (next_stree s) eqn:?. inv H.
+      eapply IHp in Heqp0.
+      simpl.
+      destruct (a =? Datatypes.length l0)%nat. eauto.
+      destruct (nth_error l0 a). reflexivity. split; auto.
+    * simpl in H. inv H. simpl.
+      destruct (a =? Datatypes.length l0)%nat eqn:H.
+      assert (nth_error l0 a = None).
+      apply nth_error_None. apply beq_nat_true in H.
+      subst. lia. rewrite H0. destruct p.
+      simpl. split. intro. inv H1. intros [H1 H2]. congruence.
+      simpl. destruct n; reflexivity.
+      destruct (nth_error l0 a); reflexivity.
+Qed.
+
+Lemma return_stree_in : forall s s' path p pos b,
+    return_stree s = Some (s',path) ->
+    stree_In b p pos s <-> stree_In b p pos s'.
+Proof.
+  induction s using stree_ind. intros.
+  destruct s. destruct o.
+  - simpl in H0. repeat destr_in H0;
+    destruct p; simpl. reflexivity.
+    destr. eapply H; eauto. simpl. auto. reflexivity.
+    destr. apply beq_nat_true in Heqb0. subst.
+    rewrite nth_error_app2. rewrite Nat.sub_diag.
+    reflexivity. lia.
+    apply beq_nat_false in Heqb0.
+    destruct (n <? Datatypes.length l0)%nat eqn:H1.
+    rewrite nth_error_app1. destr; auto.
+    apply Nat.ltb_lt. auto.
+    apply Nat.ltb_ge in H1.
+    assert (nth_error (l0++[s]) n = None).
+    apply nth_error_None.
+    rewrite app_length. simpl. lia. rewrite H0.
+    assert (nth_error l0 n = None).
+    apply nth_error_None. lia. rewrite H2.
+    reflexivity.
+  - inv H0.
+Qed.
+
+Inductive struct_eq : stree -> stree -> Prop :=
+  |struct_eq_leaf : forall fi bl1 bl2,
+      struct_eq (Node fi bl1 nil None) (Node fi bl2 nil None)
+  |struct_eq_dead_node :
+     forall fi bl1 bl2 tl1 tl2,
+       list_forall2 struct_eq tl1 tl2 ->
+       struct_eq (Node fi bl1 tl1 None) (Node fi bl2 tl2 None)
+  |struct_eq_active_node :
+     forall fi bl1 bl2 tl1 tl2 head1 head2,
+       list_forall2 struct_eq tl1 tl2 ->
+       struct_eq head1 head2 ->
+       struct_eq (Node fi bl1 tl1 (Some head1)) (Node fi bl2 tl2 (Some head2)).
+
+Theorem struct_eq_refl : forall s , struct_eq s s.
+Proof.
+  induction s using stree_ind.
+  intros. destruct s.
+  destruct o; destruct l0.
+  - apply struct_eq_active_node. constructor.
+    apply H. simpl. left. auto.
+  - apply struct_eq_active_node.
+    {
+      constructor. apply H. simpl. auto.
+      induction l0. constructor.
+      constructor. apply H. simpl. auto.
+      apply IHl0. intros. apply H.
+      simpl in H0. simpl. inv H0. auto. inv H1; auto.
+    }
+    apply H. simpl. auto.
+  - constructor.
+  - apply struct_eq_dead_node.
+    constructor. apply H. simpl. auto.
+    induction l0. constructor.
+    constructor. apply H. simpl. auto.
+    apply IHl0. intros.
+    apply H. simpl. simpl in H0.
+    destruct H0. inv H0. destruct H0; auto.
+Qed.
+
+Lemma list_forall2_struct_eq_refl : forall l,
+    list_forall2 struct_eq l l.
+Proof.
+  induction l; constructor.
+  apply struct_eq_refl. auto.
+Qed.
+
+Theorem struct_eq_comm : forall s1 s2, struct_eq s1 s2 -> struct_eq s2 s1.
+Proof.
+  induction s1 using stree_ind.
+  intros. inv H0.
+  constructor.
+  constructor.
+   eapply list_forall2_ind with (P:= fun t1 t2 => In t1 tl1 /\ struct_eq t1 t2) (P0:= fun l1 l2 => list_forall2 struct_eq l2 l1 ).
+   constructor.
+   intros. inv H0. constructor; auto. apply H. simpl. auto. auto.
+   eapply list_forall2_imply; eauto.
+  constructor.
+   eapply list_forall2_ind with (P:= fun t1 t2 => In t1 tl1 /\ struct_eq t1 t2) (P0:= fun l1 l2 => list_forall2 struct_eq l2 l1 ).
+   constructor.
+   intros. inv H0. constructor; auto. apply H. simpl. auto. auto.
+   eapply list_forall2_imply; eauto.
+   apply H. simpl. auto. auto.
+Qed.
+
+Theorem list_forall2_trans : forall {A:Type} (l2 l1 l3 : list A) (P: A -> A -> Prop),
+    (forall a1 a2 a3, In a1 l1 -> P a1 a2 -> P a2 a3 -> P a1 a3) ->
+    list_forall2 P l1 l2 ->
+    list_forall2 P l2 l3 ->
+    list_forall2 P l1 l3.
+Proof.
+  induction l2; intros; inv H0; inv H1; constructor.
+  eapply H. left. auto. all: eauto.
+  eapply IHl2. intros. exploit H. right. eauto. all: eauto.
+Qed.
+
+Theorem struct_eq_trans : forall s1 s2 s3, struct_eq s1 s2 -> struct_eq s2 s3 -> struct_eq s1 s3.
+Proof.
+  induction s1 using stree_ind.
+  intros. inv H0. inv H1.
+  - constructor.
+  - inv H5. constructor.
+  - destruct s3. inv H1. inv H2. constructor.
+    constructor.
+    eapply list_forall2_trans.
+    intros. eapply H. simpl. auto. all : eauto.
+  - destruct s3. inv H1. inv H2. constructor. inv H5. constructor.
+    eapply H; eauto. simpl. auto.
+    constructor. inv H5. constructor. eapply H; eauto. simpl. auto.
+    eapply list_forall2_trans.
+    intros. eapply H. simpl. auto. all : eauto.
+    eapply H; eauto. simpl. auto.
+Qed.
+
+Lemma next_block_stree_struct_eq: forall s path s' f pos,
+    next_block_stree s = (f,pos,path,s') -> struct_eq s s'.
+Proof.
+  induction s. intros. destruct s. destruct s'.
+  inv H0. destr_in H2.
+  destruct (next_block_stree s) eqn:?.
+  destruct p. inv H2.
+  constructor. apply list_forall2_struct_eq_refl.
+  eapply H; eauto. simpl. auto.
+  inv H2. constructor. apply list_forall2_struct_eq_refl.
+Qed.
+
+
+Definition is_active (s:stree) : Prop :=
+  match s with
+    |Node _ _ _ (Some _) => True
+    |_ => False
+  end.
+
+Lemma active_struct_eq : forall s1 s2,
+    struct_eq s1 s2 ->
+    is_active s1 <-> is_active s2.
+Proof.
+  intros. inv H; reflexivity.
+Qed.
+
+Lemma next_stree_struct_eq: forall s1 s2 id p1 p2 s1' s2',
+    struct_eq s1 s2 ->
+    next_stree s1 id = (s1',p1) ->
+    next_stree s2 id = (s2',p2) ->
+    p1 = p2 /\ struct_eq s1' s2'.
+Proof.
+  induction s1. intros.
+  destruct s1; destruct s2. inv H0.
+  - inv H1. inv H2. split. auto. constructor. constructor. constructor.
+  - inv H1. inv H2. split.
+    apply list_forall2_length in H4. congruence.
+    constructor. auto. constructor.
+  - inv H1. inv H2. destr_in H3. destr_in H1.
+    inv H3. inv H1.
+    apply list_forall2_length in H5 as H6.
+    exploit H; eauto. simpl. auto. intros [H1 H2].
+    split. congruence. constructor. auto. auto.
+Qed.
+
+Lemma return_stree_struct_eq: forall s1 s2 s1' p,
+    struct_eq s1 s2 ->
+    return_stree s1 = Some (s1',p) ->
+    exists s2',
+    return_stree s2 = Some (s2',p) /\
+    struct_eq s1' s2'.
+Proof.
+  induction s1. intros.
+  destruct s1; destruct s2. inv H0; inv H1.
+  repeat destr_in H2.
+  + exploit H; eauto. simpl. auto. intros (head2' & H5 & H6).
+    exists (Node f0 l1 l2 (Some head2')). split. simpl. rewrite H5.
+    apply list_forall2_length in H4 as H7. rewrite H7. auto.
+    constructor. auto. auto.
+  + exists (Node f0 l1 (l2++[head2]) None). split.
+    simpl. destruct head1. inv Heqo. repeat destr_in H1.
+    inv H11. simpl. apply list_forall2_length in H4 as H7. rewrite H7. auto.
+    simpl. apply list_forall2_length in H4 as H7. rewrite H7. auto.
+    constructor. apply list_forall2_app. auto.
+    constructor. auto. constructor.
+Qed.
+
+Lemma struct_eq_next_block_stree : forall s1 s2 fid1 fid2 p1 p2 pos1 pos2 s1' s2',
+    struct_eq s1 s2 ->
+    next_block_stree s1 = (fid1,pos1,p1,s1') ->
+    next_block_stree s2 = (fid2,pos2,p2,s2') ->
+    fid1=fid2 /\ p1 = p2.
+Proof.
+  induction s1. intros.
+  destruct s1. destruct s2. inv H0.
+  - inv H1. inv H2. auto.
+  - inv H1. inv H2. auto.
+  - inv H1. inv H2.  repeat destr_in H3.  repeat destr_in H1.
+    exploit H; eauto. simpl. auto. intros [X Y].
+    split. auto. subst. erewrite list_forall2_length; eauto.
+Qed.
+
+End STREE.
+
+Module StrucMem.
+Include Mem(Struc_Block).
+Import Struc_Block.
+
+Record struc' : Type := mkstruc {
+  stack : stree;
+  global : list ident;
+}.
+
+Definition struc := struc'.
+
+Definition struc_empty : struc := mkstruc empty_stree nil.
+
+Definition struc_cpath (s:struc) := cpath (stack s).
+
+Definition struc_npath (s:struc) := npath (stack s).
+
+Definition struc_depth (s:struc) := depth (stack s).
+
+Definition struc_In(b:block)(s:struc) : Prop :=
+  match b with
+  | Stack fid path pos => stree_In fid path pos (stack s)
+  | Global id => In id (global s)
+  end.
+
+Definition empty_in: forall b, ~ struc_In b struc_empty.
+Proof.
+  intros. destruct b; simpl in *; try congruence.
+  destruct p; unfold stree_In; simpl; auto. intro. inv H. auto.
+  destruct n; auto.
+Qed.
+
+Definition struc_dec : forall b s, {struc_In b s}+{~struc_In b s}.
+Proof.
+  intros. destruct b.
+  apply stree_Indec.
+  apply In_dec. apply peq.
+Qed.
+
+Definition fresh_block (s:struc): block :=
+  match next_block_stree (stack s) with
+    |(f,pos,path,_) =>  Stack f path pos
+  end.
+
+Theorem freshness : forall s, ~struc_In (fresh_block s) s.
+Proof.
+  intros. unfold fresh_block.
+  destruct (next_block_stree (stack s)) eqn:?.
+  destruct p. destruct p.
+  eapply stree_freshness; eauto.
+Qed.
+
+Definition struc_incr (s:struc):struc :=
+  let (pp,t') := next_block_stree (stack s) in
+  mkstruc t' (global s).
+
+Definition struc_include(s1 s2:struc) := forall b, struc_In b s1 -> struc_In b s2.
+
+Theorem struc_incr_in : forall b s,
+    struc_In b (struc_incr s) <-> b = (fresh_block s) \/ struc_In b s.
+Proof.
+  intros. unfold struc_In. destruct b.
+  - unfold struc_incr. unfold fresh_block.
+    destruct (next_block_stree) eqn:?. simpl.
+    destruct p1. destruct p1.
+    eapply next_block_stree_in in Heqp1.
+    split. intro. apply Heqp1 in H. destruct H.
+    inv H. auto. auto.
+    intro. apply Heqp1. destruct H.
+    inv H. auto. auto.
+  - unfold struc_incr. unfold fresh_block.
+    destruct (next_block_stree) eqn:?. simpl.
+    destruct p. destruct p. split.
+    auto. intros [H|H]. inv H. auto.
+Qed.
+
+Theorem struc_incr_in1 : forall s, struc_In (fresh_block s) (struc_incr s).
+Proof. intros. apply struc_incr_in. left. auto. Qed.
+Theorem struc_incr_in2 : forall s, struc_include s (struc_incr s).
+Proof. intros. intro. intro. apply struc_incr_in. right. auto. Qed.
+
+Lemma struc_include_refl : forall s:struc, struc_include s s.
+Proof. intro. intro. auto. Qed.
+
+Lemma struc_include_trans:
+  forall p q r:struc,struc_include p q-> struc_include q r -> struc_include p r.
+Proof.
+  intros. intro. intro.  auto.
+Qed.
+
+Lemma struc_include_incr:
+  forall s, struc_include s (struc_incr s).
+Proof.
+  intros. apply struc_incr_in2.
+Qed.
+
+(* struc_incr_frame *)
+Definition struc_incr_frame (s:struc)(id:ident):struc :=
+  let (t',p) := next_stree (stack s) id in
+  mkstruc t' (global s).
+
+Theorem struc_incr_frame_in : forall s b id,
+    struc_In b s <-> struc_In b (struc_incr_frame s id).
+Proof.
+  intros. unfold struc_In. destruct b.
+  - unfold struc_incr_frame.
+    destruct (next_stree (stack s)) eqn:?.
+    simpl.
+    eapply next_stree_in. eauto.
+  - unfold struc_incr_frame.
+    destruct (next_stree (stack s)).
+    reflexivity.
+Qed.
+
+(* struc_return_frame *)
+Definition struc_return_frame (s:struc) : option struc :=
+  match return_stree (stack s) with
+    |Some (t',p) => Some (mkstruc t' (global s))
+    |None => None
+  end.
+
+Definition struc_return_frame' (s:struc) : struc :=
+  match struc_return_frame s with
+    |Some s' => s'
+    |None => struc_empty
+  end.
+
+Lemma struc_return_refl : forall s s', is_active (stack s) ->
+    struc_return_frame s = Some s' <-> struc_return_frame' s = s'.
+Proof.
+  intros.
+  unfold struc_return_frame'. destruct (struc_return_frame s) eqn:?.
+  split;  congruence.
+  unfold struc_return_frame in Heqo.
+  destruct (return_stree (stack s)) eqn:?. destruct p.
+  inv Heqo.
+  unfold is_active in H. destruct (stack s).
+  destruct o.
+  inv Heqo0. destr_in H1. destruct p. inv H1.
+  destruct H.
+Qed.
+
+Lemma struc_return_refl' : forall s , is_active (stack s) ->
+    struc_return_frame s = Some (struc_return_frame' s).
+Proof.
+  intros. apply struc_return_refl; auto.
+Qed.
+
+Theorem struc_return_frame_in : forall s s',
+    struc_return_frame s = Some (s') ->
+    (forall b, struc_In b s <-> struc_In b s').
+Proof.
+  intros.
+  destruct b; unfold struc_return_frame in H;
+  destruct (return_stree (stack s)) eqn:?.
+  - destruct p1. inv H.
+    simpl.
+    eapply return_stree_in; eauto.
+  - inv H.
+  - destruct p. inv H. reflexivity.
+  - inv H.
+Qed.
+
+(* struc_incr_glob *)
+Definition struc_incr_glob (i:ident) (s:struc) : struc :=
+ mkstruc (stack s) (i::(global s)).
+
+Theorem struc_incr_glob_in :  forall i s b,
+    struc_In b (struc_incr_glob i s) <-> b = (Global i) \/ struc_In b s.
+Proof.
+  split.
+  - unfold struc_incr_glob.
+    destruct b; simpl. auto. intros [H|H]. rewrite H. auto. auto.
+  - intros [H|H]; unfold struc_incr_glob.
+    rewrite H. simpl. auto.
+    destruct b. simpl. auto. simpl. auto.
+Qed.
+
+Theorem struc_incr_glob_in1 : forall i s, struc_In (Global i) (struc_incr_glob i s).
+Proof. intros. apply struc_incr_glob_in. left. auto. Qed.
+Theorem struc_incr_glob_in2 : forall i s, struc_include s (struc_incr_glob i s).
+Proof. intros. intro. intro. apply struc_incr_glob_in. right. auto. Qed.
+
+Definition match_struc_sup (s:struc) (m:mem) : Prop :=
+  forall b, struc_In b s <-> In b (support m).
+
+Record mems : Type := mkmems{
+  structure : struc;
+  memory: mem;
+  match_struc_mem : match_struc_sup structure memory
+}.
+
+Program Definition mems_empty := mkmems struc_empty empty _.
+Next Obligation.
+intro. simpl. generalize empty_in.
+intro. split. intro. apply H in H0. auto. intro. inversion H0.
+Qed.
+
+End StrucMem.
+
+
+
+
+
 
